some more progress

lib/Marshalling/TupleMarshalling.i.dfy
@@ -214,32 +214,32 @@ abstract module Tuple3Marshalling refines Marshalling {
 
   predicate parsable(data: mseq<byte>)
   {
-    && var tableEnd := sizeOfTable();
-    && tableEnd < Uint64UpperBound()
-    && |data| >= tableEnd
-    && TableMarshalling.parsable(data[..tableEnd])
-    && var table :mseq<Boundary> := TableMarshalling.parse(data[..tableEnd]);
+    && var tableSize := sizeOfTable();
+    && tableSize < Uint64UpperBound()
+    && |data| >= tableSize
+    && TableMarshalling.parsable(data[..tableSize])
+    && var table :mseq<Boundary> := TableMarshalling.parse(data[..tableSize]);
 
-    && var end0 := BoundaryInt.toInt(table[0]);
-    && tableEnd <= end0 <= |data|
-    && ElemMarshalling0.parsable(data[tableEnd..end0])
+    && var bound0 := BoundaryInt.toInt(table[0]);
+    && tableSize <= bound0 <= |data|
+    && ElemMarshalling0.parsable(data[tableSize..bound0])
 
-    && var end1 := BoundaryInt.toInt(table[1]);
-    && end0 <= end1 <= |data|
-    && ElemMarshalling1.parsable(data[end0..end1])
+    && var bound1 := BoundaryInt.toInt(table[1]);
+    && bound0 <= bound1 <= |data|
+    && ElemMarshalling1.parsable(data[bound0..bound1])
 
-    && ElemMarshalling2.parsable(data[end1..])
+    && ElemMarshalling2.parsable(data[bound1..])
   }
 
   function parse(data: mseq<byte>) : UnmarshalledType
   {
-    var tableEnd := sizeOfTable();
-    var table :mseq<Boundary> := TableMarshalling.parse(data[..tableEnd]);
-    var end0 :=  BoundaryInt.toInt(table[0]);
-    var end1 :=  BoundaryInt.toInt(table[1]);
-    var elem0 := ElemMarshalling0.parse(data[tableEnd..end0]);
-    var elem1 := ElemMarshalling1.parse(data[end0..end1]);
-    var elem2 := ElemMarshalling2.parse(data[end1..]);
+    var tableSize := sizeOfTable();
+    var table :mseq<Boundary> := TableMarshalling.parse(data[..tableSize]);
+    var bound0 := BoundaryInt.toInt(table[0]);
+    var bound1 := BoundaryInt.toInt(table[1]);
+    var elem0 := ElemMarshalling0.parse(data[tableSize..bound0]);
+    var elem1 := ElemMarshalling1.parse(data[bound0..bound1]);
+    var elem2 := ElemMarshalling2.parse(data[bound1..]);
     (elem0, elem1, elem2)
   }
 
@@ -251,13 +251,13 @@ abstract module Tuple3Marshalling refines Marshalling {
       return None;
     }
 
-    var tableEnd := entrySize * 2;
+    var tableSize := entrySize * 2;
 
-    if tableEnd > |data| as uint64 {
+    if tableSize > |data| as uint64 {
       return None;
     }
 
-    var tableOpt := TableMarshalling.TryParse(data[..tableEnd]);
+    var tableOpt := TableMarshalling.TryParse(data[..tableSize]);
     
     if tableOpt.None? {
       return None;
@@ -270,20 +270,20 @@ abstract module Tuple3Marshalling refines Marshalling {
       return None;
     }
 
-    var end0 := BoundaryInt.toUint64(table[0]);
-    var end1 := BoundaryInt.toUint64(table[1]);
+    var bound0 := BoundaryInt.toUint64(table[0]);
+    var bound1 := BoundaryInt.toUint64(table[1]);
 
-    if end0 > |data| as uint64 || end0 < tableEnd {
+    if bound0 > |data| as uint64 || bound0 < tableSize {
       return None;
     }
 
-    if end1 > |data| as uint64 || end1 < end0 {
+    if bound1 > |data| as uint64 || bound1 < bound0 {
       return None;
     }
 
-    var elemOpt0 := ElemMarshalling0.TryParse(data[tableEnd..end0]);
-    var elemOpt1 := ElemMarshalling1.TryParse(data[end0..end1]);
-    var elemOpt2 := ElemMarshalling2.TryParse(data[end1..]);
+    var elemOpt0 := ElemMarshalling0.TryParse(data[tableSize..bound0]);
+    var elemOpt1 := ElemMarshalling1.TryParse(data[bound0..bound1]);
+    var elemOpt2 := ElemMarshalling2.TryParse(data[bound1..]);
 
     if elemOpt0.None? || elemOpt1.None? || elemOpt2.None? {
       return None;
@@ -300,13 +300,13 @@ abstract module Tuple3Marshalling refines Marshalling {
       return false;
     }
 
-    var tableEnd := sizeOfTable() as uint64;
+    var tableSize := sizeOfTable() as uint64;
 
-    if tableEnd > |data| as uint64 {
+    if tableSize > |data| as uint64 {
       return false;
     }
 
-    var tableOpt := TableMarshalling.TryParse(data[..tableEnd]);
+    var tableOpt := TableMarshalling.TryParse(data[..tableSize]);
     
     if tableOpt.None? {
       return false;
@@ -319,20 +319,20 @@ abstract module Tuple3Marshalling refines Marshalling {
       return false;
     }
 
-    var end0 := BoundaryInt.toUint64(table[0]);
-    var end1 := BoundaryInt.toUint64(table[1]);
+    var bound0 := BoundaryInt.toUint64(table[0]);
+    var bound1 := BoundaryInt.toUint64(table[1]);
 
-    if end0 > |data| as uint64 || end0 < tableEnd {
+    if bound0 > |data| as uint64 || bound0 < tableSize {
       return false;
     }
 
-    if end1 > |data| as uint64 || end1 < end0 {
+    if bound1 > |data| as uint64 || bound1 < bound0 {
       return false;
     }
 
-    var elemParsable0 := ElemMarshalling0.Parsable(data[tableEnd..end0]);
-    var elemParsable1 := ElemMarshalling1.Parsable(data[end0..end1]);
-    var elemParsable2 := ElemMarshalling2.Parsable(data[end1..]);
+    var elemParsable0 := ElemMarshalling0.Parsable(data[tableSize..bound0]);
+    var elemParsable1 := ElemMarshalling1.Parsable(data[bound0..bound1]);
+    var elemParsable2 := ElemMarshalling2.Parsable(data[bound1..]);
 
     if !elemParsable0 || !elemParsable1 || !elemParsable2 {
       return false;
@@ -343,15 +343,15 @@ abstract module Tuple3Marshalling refines Marshalling {
 
   method Parse(data: mseq<byte>) returns (value: UnmarshalledType)
   {
-    var tableEnd := sizeOfTable() as uint64;
-    var table :mseq<Boundary> := TableMarshalling.Parse(data[..tableEnd]);
+    var tableSize := sizeOfTable() as uint64;
+    var table :mseq<Boundary> := TableMarshalling.Parse(data[..tableSize]);
   
-    var end0 := BoundaryInt.toUint64(table[0]);
-    var end1 := BoundaryInt.toUint64(table[1]);
+    var bound0 := BoundaryInt.toUint64(table[0]);
+    var bound1 := BoundaryInt.toUint64(table[1]);
 
-    var elem0 := ElemMarshalling0.Parse(data[tableEnd..end0]);
-    var elem1 := ElemMarshalling1.Parse(data[end0..end1]);
-    var elem2 := ElemMarshalling2.Parse(data[end1..]);
+    var elem0 := ElemMarshalling0.Parse(data[tableSize..bound0]);
+    var elem1 := ElemMarshalling1.Parse(data[bound0..bound1]);
+    var elem2 := ElemMarshalling2.Parse(data[bound1..]);
     return (elem0, elem1, elem2);
   }
 
@@ -361,15 +361,81 @@ abstract module Tuple3Marshalling refines Marshalling {
     && ElemMarshalling0.marshallable(elem0)
     && ElemMarshalling1.marshallable(elem1)
     && ElemMarshalling2.marshallable(elem2)
-    && var tableEnd := sizeOfTable();
+    && var tableSize := sizeOfTable();
     var size0 := ElemMarshalling0.size(elem0);
     var size1 := ElemMarshalling1.size(elem1);
-    var end0 := tableEnd + size0;
-    var end1 := end0 + size1;
-    && BoundaryInt.MinValue() <= end0 < BoundaryInt.UpperBound()
-    && BoundaryInt.MinValue() <= end1 < BoundaryInt.UpperBound()
-    && var table := [BoundaryInt.fromInt(end0), BoundaryInt.fromInt(end1)];
+    var bound0 := tableSize + size0;
+    var bound1 := bound0 + size1;
+    && BoundaryInt.MinValue() <= bound0 < BoundaryInt.UpperBound()
+    && BoundaryInt.MinValue() <= bound1 < BoundaryInt.UpperBound()
+    && var table := [BoundaryInt.fromInt(bound0), BoundaryInt.fromInt(bound1)];
     && TableMarshalling.marshallable(table)
   }
 
+  function size(value: UnmarshalledType) : nat
+  {
+    var (elem0, elem1, elem2) := value;
+    var tableSize := sizeOfTable();
+    var size0 := ElemMarshalling0.size(elem0);
+    var size1 := ElemMarshalling1.size(elem1);
+    var size2 := ElemMarshalling2.size(elem2);
+    tableSize + size0 + size1 + size2
+  }
+
+  method Size(value: UnmarshalledType) returns (sz: uint64)
+  {
+    var (elem0, elem1, elem2) := value;
+    var tableSize := sizeOfTable() as uint64;
+    var size0 := ElemMarshalling0.Size(elem0);
+    var size1 := ElemMarshalling1.Size(elem1);
+    var size2 := ElemMarshalling2.Size(elem2);
+    sz := tableSize + size0 + size1 + size2;
+  }
+
+  method Marshall(value: UnmarshalledType, linear data: mseq<byte>, start: uint64)
+    returns (linear newdata: mseq<byte>, end: uint64)
+  {
+    var (elem0, elem1, elem2) := value;
+    var tableSize := sizeOfTable() as uint64;
+
+    var size0 := ElemMarshalling0.Size(elem0);
+    var size1 := ElemMarshalling1.Size(elem1);
+
+    var bound0 := tableSize + size0;
+    var bound1 := bound0 + size1;
+
+    var table := [BoundaryInt.fromUint64(bound0), BoundaryInt.fromUint64(bound1)];
+
+    newdata, end := TableMarshalling.Marshall(table, data, start);
+    ghost var newdata0 :seq<byte>, end0 := newdata, end;
+
+    newdata, end := ElemMarshalling0.Marshall(elem0, newdata, end);
+    ghost var newdata1 :seq<byte>, end1 := newdata, end;
+
+    newdata, end := ElemMarshalling1.Marshall(elem1, newdata, end);
+    ghost var newdata2 :seq<byte>, end2 := newdata, end;
+
+    newdata, end := ElemMarshalling2.Marshall(elem2, newdata, end);
+
+    assert BoundaryInt.toInt(table[0]) == bound0 as int by {
+      BoundaryInt.fromtoInverses();
+    }
+    assume BoundaryInt.toInt(table[1]) == bound1 as int;
+
+    assert newdata[start..end][..tableSize] == newdata[start..end0] == newdata0[start..end0];
+    assert TableMarshalling.parse(newdata[start..end0]) == table;
+    
+    assert newdata[start..end][tableSize..bound0] == newdata[end0..end1] ==  newdata1[end0..end1] by {
+      Sequences.lemma_seq_slice_slice(newdata, start as int, end as int, tableSize as int, bound0 as int);
+    }
+    assert ElemMarshalling0.parse(newdata[end0..end1]) == elem0;
+
+    assert newdata[start..end][bound0..bound1] == newdata[end1..end2] == newdata2[end1..end2] by {
+      Sequences.lemma_seq_slice_slice(newdata, start as int, end as int, bound0 as int, bound1 as int);
+    }
+    assert ElemMarshalling1.parse(newdata[end1..end2]) == elem1;
+
+    assert newdata[start..end][bound1..] == newdata[end2..end];
+    assert ElemMarshalling2.parse(newdata[end2..end]) == elem2;
+  }
 }
